proof that evaluation is continuous.

cs/classical_func.v
@@ -30,33 +30,101 @@ Proof. done. Qed.
 
 Require Import ClassicalChoice.
 
+Fixpoint collect_left S T (L: seq (S + T)) := match L with
+                      | nil => nil
+                      | a :: L' => match a with
+                                   | inl b => b :: (collect_left L')
+                                   | inr _ => collect_left L'
+                                   end
+                      end.
 
-(*
-Lemma eval_rlzr_cntop (X Y: cs):
-  (@eval_rlzr (questions X) (questions Y) (answers X) (answers Y)) \is_continuous_operator.
+Fixpoint collect_right S T (L: seq (S + T)) := match L with
+                      | nil => nil
+                      | a :: L' => match a with
+                                   | inr b => b :: (collect_right L')
+                                   | inl _ => collect_right L'
+                                   end
+                      end.
+
+Lemma prod_cntop_left (X Y Z: cs) (F: names (X \*_cs Y) ->> names Z) phi:
+  F \is_continuous_operator ->
+  (make_mf (fun psi Fphipsi => F (name_pair phi psi) Fphipsi)) \is_continuous_operator.
 Proof.
-move => psiphi [Fphi /eval_rlzr_val FphiFphi].
-have [ | mf mod]:= @FM_cont _ _ _ _ (lprj psiphi) (rprj psiphi); first by exists Fphi.
-have [ | mf' mod']:= @FM_val_cont _ _ _ _ (rprj psiphi) (lprj psiphi); first by exists Fphi.
-exists (fun q' => (map inl (mf' q')) ++ (map inr (mf q'))) => q'.
-exists (Fphi q') => psi'phi' /coin_agre /coin_cat [coin' coin] Fphi'/eval_rlzr_val Fphi'Fphi'.
-pose psi'phi := name_pair (lprj psi'phi') (rprj psiphi).
-have : psi'phi \from dom (eval_rlzr).
-rewrite /=.
-suff prp: forall q, exists a, exists c, M (lprj psi'phi) c (rprj psi'phi) q = Some a.
-- by have [fasdf prp']:= choice _ prp; exists fasdf; apply prp'.
-move => q.
-exists 
-have [a' crt']:= mod q'.
-have crt:= cert_icf FphiFphi crt'; move: a' crt' => _ _.
-apply/crt.
-elim: (mf q') coin => [_ crt | ].
+move => cont psi [Fphipsi /= val].
+have [ | mf mod]:= cont (name_pair phi psi); first by exists Fphipsi.
+exists (fun q => collect_right (mf q)) => q.
+exists (Fphipsi q) => psi' /coin_agre coin Fphipsi' val'.
+have [a' crt]:= mod q; apply/(cert_icf val crt)/val'/coin_agre.
+by elim: (mf q) coin => // [[q' L ih /=/ih | q' L ih /= [-> /ih]]].
+Qed.
 
-rewrite /=.
-pose psiphi' := name_pair (lprj psiphi) (rprj psi'phi').
+Lemma prod_cntop_right (X Y Z: cs) (F: names (X \*_cs Y) ->> names Z) psi:
+  F \is_continuous_operator ->
+  (make_mf (fun phi Fphipsi => F (name_pair phi psi) Fphipsi)) \is_continuous_operator.
+Proof.
+move => cont phi [Fphipsi /= val].
+have [ | mf mod]:= cont (name_pair phi psi); first by exists Fphipsi.
+exists (fun q => collect_left (mf q)) => q.
+exists (Fphipsi q) => psi' /coin_agre coin Fphipsi' val'.
+have [a' crt]:= mod q; apply/(cert_icf val crt)/val'/coin_agre.
+by elim: (mf q) coin => // [[q' L ih /= [-> /ih] | q' L ih /= /ih]].
+Qed.
 
-have [b' crt']:= mod' q'.
-have: Fphi' q' = b'.
-- apply/(crt' (lprj psiphi) _ Fphi').
-  exact/agre_ref.
-  rewrite /=.*)
+Definition name_pairs (X Y: cs) := make_subset (fun phipsi =>
+       exists (phi: names X), exists (psi: names Y), phipsi = name_pair phi psi).
+
+Lemma eval_rlzr_cntop (X Y: cs):
+  (@eval_rlzr (questions X) (questions Y) (answers X) (answers Y))|_(dom (rep (X c-> Y \*_cs X))) \is_continuous_operator.
+Proof.
+move => psiphi [Fpsiphi [[[f x] [psinf phinx]] /eval_rlzr_val val]].
+rewrite /= in psinf phinx; have phifd: (rprj psiphi) \from dom \F_(M (lprj psiphi)) by exists Fpsiphi.
+have [mf [Lf prp]]:= FM_ucont (lprj psiphi).
+exists (fun q' => map inl (Lf (rprj psiphi) q') ++ map inr (mf (rprj psiphi) q')) => q'.
+exists (Fpsiphi q') => psi'phi' /coin_agre/coin_cat[coin coin'].
+have : (rprj psiphi) \and (rprj psi'phi') \coincide_on (mf (rprj psiphi) q').
+- by elim: (mf (rprj psiphi) q') coin' => // q K ih /= [eq /ih]; split; first rewrite /rprj eq.
+have: (lprj psiphi) \and (lprj psi'phi') \coincide_on (Lf (rprj psiphi) q').
+- by elim: (Lf (rprj psiphi) q') coin => // q K ih /= [eq /ih]; split; first rewrite /lprj eq.
+move: coin coin' => _ _ coin coin'.
+rewrite det_restr => [[[f' x'] [psi'nf' phi'nx']]] Fpsi'phi'/eval_rlzr_val val'.
+rewrite /= in psi'nf' phi'nx'; pose psiphi':= name_pair (lprj psiphi) (rprj psi'phi').
+have psiphi'nfx': psiphi' \is_description_of ((f, x'): X c-> Y \*_cs X).
+- by trivial.
+have [Fpsiphi' val'']: psiphi' \from dom eval_rlzr.
+- by have []:= eval_rlzr_crct psiphi'nfx'; first exact/F2MF_dom.
+have [ | mod _]:= prp (rprj psiphi); first by exists Fpsiphi.
+have [a' tempcrt]:= mod q'.  
+have crt := cert_icf val tempcrt _; move: a' tempcrt => _ _.
+rewrite -(crt (rprj psi'phi') _ Fpsiphi' val''); last first.
+- apply/coin_agre/coin'.
+have mfeq: mf (rprj psiphi) q' = mf (rprj psi'phi') q'.
+- have [ | _ [mod' _]]:= prp (rprj psiphi); first by exists Fpsiphi.
+  have [a' crt']:= mod' q'.
+  suff ->: mf (rprj psi'phi') q' = a' by apply/crt'; [exact/agre_ref | split; first exists Fpsiphi].
+  apply/crt'; first by apply/coin_agre/coin'.
+  split => //; apply/rlzr_dom; first exact/ psinf.
+  - apply/phi'nx'.
+  exact/F2MF_tot.
+have eq: Lf (rprj psiphi) q' = Lf (rprj psi'phi') q'.
+- have [ | _ [_ [mod' _]]]:= prp (rprj psi'phi'); first by exists Fpsiphi'.
+  have [a' crt']:= mod' q'.
+  have ->: Lf (rprj psiphi) q' = a'.
+  - by apply/crt'; first by apply/coin_agre; rewrite -mfeq; exact/coin_sym/coin'.
+  symmetry.
+  apply/crt'; first exact/agre_ref; split => //.
+  apply/rlzr_dom; first exact/psinf; first exact/phi'nx'; exact/F2MF_tot.
+have [ | _ [_ [_ mod']]] := prp (rprj psi'phi'); first by exists Fpsiphi'.
+have [a' crt']:= mod' q'.
+suff ->: Fpsi'phi' q' = a' by symmetry; apply/crt'; first exact/agre_ref.
+by apply/crt'; first by apply/coin_agre; rewrite -eq; exact/coin.
+Qed.
+
+Lemma eval_cont (X Y: cs): (@evaluation X Y) \is_continuous.
+Proof.
+exists (@eval_rlzr (questions X) (questions Y) (answers X) (answers Y))|_(dom (rep (X c-> Y \*_cs X))).
+split; last exact/eval_rlzr_cntop.
+rewrite rlzr_F2MF => psiphi fx psiphinfx.
+have [ | [Fpsiphi val] prp]:= eval_rlzr_crct psiphinfx; first exact/F2MF_dom.
+split => [ | Fq [_ val']]; first by exists Fpsiphi; split; first by exists fx.
+by have [f'x' [nm ->]]:= prp Fq val'.                         
+Qed.
